Added glue code including parsing & conversion

Simple_Networks/Simple_Network_Language_Export_Code.thy
@@ -1,8 +1,9 @@
 theory Simple_Network_Language_Export_Code
   imports
+    "../../Parser_Combinators/JSON_Parsing"
     Simple_Network_Language_Renaming
     "../UPPAAL_State_Networks_Impl_Refine_Calc"
-    "../library/Error_Monad"
+    "../library/Error_List_Monad"
 begin
 
 datatype result =
@@ -14,9 +15,9 @@ hide_const m
 
 locale Simple_Network_Rename_Formula_String =
   Simple_Network_Rename_Defs where automata = automata for automata ::
-    "(String.literal list \<times>
-     (String.literal act, String.literal, String.literal, int, String.literal, int) transition list
-      \<times> (String.literal \<times> (String.literal, int) cconstraint) list) list" +
+    "(nat list \<times>
+     (String.literal act, nat, String.literal, int, String.literal, int) transition list
+      \<times> (nat \<times> (String.literal, int) cconstraint) list) list" +
   assumes renum_states_inj:
     "\<forall>i<n_ps. \<forall>x\<in>loc_set. \<forall>y\<in>loc_set. renum_states i x = renum_states i y \<longrightarrow> x = y"
   and renum_clocks_inj: "inj_on renum_clocks clk_set'"
@@ -24,13 +25,13 @@ locale Simple_Network_Rename_Formula_String =
   and bounds'_var_set: "fst ` set bounds' \<subseteq> var_set"
   and loc_set_invs: "\<Union> ((\<lambda>g. fst ` set g) ` set (map (snd o snd) automata)) \<subseteq> loc_set"
   and loc_set_broadcast: "\<Union> ((set o fst) ` set automata) \<subseteq> loc_set"
-  fixes \<Phi> :: "(String.literal, String.literal, int) formula"
+  fixes \<Phi> :: "(nat, nat, String.literal, int) formula"
     and s\<^sub>0 :: "(String.literal \<times> int) list"
-    and L\<^sub>0 :: "String.literal list"
+    and L\<^sub>0 :: "nat list"
   assumes L\<^sub>0_states: "L\<^sub>0 \<in> states"
       and s\<^sub>0_dom: "fst ` set s\<^sub>0 = var_set" and s\<^sub>0_distinct: "distinct (map fst s\<^sub>0)"
   assumes formula_dom:
-    "set1_formula \<Phi> \<subseteq> loc_set"
+    "set2_formula \<Phi> \<subseteq> loc_set"
     "locs_of_formula \<Phi> \<subseteq> {0..<n_ps}"
     "vars_of_formula \<Phi> \<subseteq> var_set"
 begin
@@ -38,7 +39,7 @@ begin
 interpretation Simple_Network_Rename_Formula
   by (standard; 
       rule renum_states_inj renum_clocks_inj renum_vars_inj bounds'_var_set
-      loc_set_invs loc_set_broadcast infinite_literal
+      loc_set_invs loc_set_broadcast infinite_literal infinite_UNIV_nat
       L\<^sub>0_states s\<^sub>0_dom s\<^sub>0_distinct formula_dom)
 
 lemmas Simple_Network_Rename_intro = Simple_Network_Rename_Formula_axioms
@@ -417,7 +418,6 @@ definition
 
 
 paragraph \<open>Unsafe Glue Code\<close>
-
 definition list_of_set :: "'a set \<Rightarrow> 'a list" where
   "list_of_set xs = undefined"
 
@@ -425,15 +425,10 @@ code_printing
   constant list_of_set \<rightharpoonup> (SML) "(fn Set xs => xs) _"
        and              (OCaml) "(fun x -> match x with Set xs -> xs) _"
 
-definition print :: "String.literal \<Rightarrow> unit" where
-  "print x = ()"
 
-code_printing
-  constant print \<rightharpoonup> (SML) "print _"
-       and        (OCaml) "print'_string _"
 
-definition println :: "String.literal \<Rightarrow> unit" where
-  "println x = print (x + STR ''\<newline>'')"
+definition
+  "mk_renaming' xs \<equiv> mk_renaming (String.implode o show) xs"
 
 definition "make_renaming \<equiv> \<lambda> broadcast automata bounds.
   let
@@ -451,7 +446,7 @@ definition "make_renaming \<equiv> \<lambda> broadcast automata bounds.
   in do {
     (renum_acts, renum_clocks, renum_vars) \<leftarrow>
       mk_renaming action_set <|> mk_renaming clk_set <|> mk_renaming var_set;
-    renum_states_list \<leftarrow> combine_map (\<lambda>i. mk_renaming (loc_set i)) [0..<n_ps];
+    renum_states_list \<leftarrow> combine_map (\<lambda>i. mk_renaming' (loc_set i)) [0..<n_ps];
     let renum_states = (\<lambda>i. renum_states_list ! i);
     Result (m, num_states, num_actions, renum_acts, renum_vars, renum_clocks, renum_states)
   }"
@@ -470,18 +465,21 @@ definition "preproc_mc \<equiv> \<lambda> (broadcast, automata, bounds) L\<^sub>
 "
 
 definition
-"main \<equiv> \<lambda> (broadcast, automata, bounds) L\<^sub>0 s\<^sub>0 formula. do {
+  "err s = Error [s]"
+
+definition
+"do_preproc_mc \<equiv> \<lambda> (broadcast, automata, bounds) L\<^sub>0 s\<^sub>0 formula. do {
   r \<leftarrow> preproc_mc (broadcast, automata, bounds) L\<^sub>0 s\<^sub>0 formula;
   return (case r of
     Error es \<Rightarrow>
       intersperse (STR ''\<newline>'') es
       |> concat_str
       |> (\<lambda>e. STR ''Error during preprocessing:\<newline>'' + e)
-      |> println
-  | Result Renaming_Failed \<Rightarrow> STR ''Renaming failed'' |> println
-  | Result Preconds_Unsat \<Rightarrow>  STR ''Input invalid'' |> println
-  | Result Unsat \<Rightarrow> STR ''Property is not satisfied!'' |> println
-  | Result Sat   \<Rightarrow> STR ''Property is satisfied!'' |> println
+      |> err
+  | Result Renaming_Failed \<Rightarrow> STR ''Renaming failed'' |> err
+  | Result Preconds_Unsat \<Rightarrow> STR ''Input invalid'' |> err
+  | Result Unsat \<Rightarrow> STR ''Property is not satisfied!'' |> Result
+  | Result Sat   \<Rightarrow> STR ''Property is satisfied!'' |> Result
   )
 }"
 
@@ -489,6 +487,429 @@ lemmas [code] =
   Simple_Network_Impl.action_set_def
   Simple_Network_Impl.loc_set'_def
 
-export_code main in SML module_name Main
+export_code do_preproc_mc in SML module_name Main
+
+definition parse where
+  "parse parser s \<equiv> case parse_all lx_ws parser s of
+    Inl e \<Rightarrow> Error [e () ''Parser: '' |> String.implode]
+  | Inr r \<Rightarrow> Result r"
+
+definition get_nat :: "string \<Rightarrow> JSON \<Rightarrow> nat Error_List_Monad.result" where
+  "get_nat s json \<equiv> case json of
+    Object as \<Rightarrow> Error []
+  | _ \<Rightarrow> Error [STR ''JSON Get: expected object'']
+" for json
+
+definition of_object :: "JSON \<Rightarrow> (string \<rightharpoonup> JSON) Error_List_Monad.result" where
+  "of_object json \<equiv> case json of
+    Object as \<Rightarrow> map_of as |> Result
+  | _ \<Rightarrow> Error [STR ''json_to_map: expected object'']
+" for json
+
+definition get where
+  "get m x \<equiv> case m x of None \<Rightarrow> Error [STR ''Get: key not found''] | Some a \<Rightarrow> Result a"
+
+definition
+  "get_default def m x \<equiv> case m x of None \<Rightarrow> def | Some a \<Rightarrow> a"
+
+definition default where
+  "default def x \<equiv> case x of Result s \<Rightarrow> s | Error e \<Rightarrow> def"
+
+definition of_array where
+  "of_array json \<equiv> case json of
+    JSON.Array s \<Rightarrow> Result s
+  | _ \<Rightarrow> Error [STR ''of_array: expected sequence'']
+" for json
+
+definition of_string where
+  "of_string json \<equiv> case json of
+    JSON.String s \<Rightarrow> Result (String.implode s)
+  | _ \<Rightarrow> Error [STR ''of_array: expected sequence'']
+" for json
+
+definition of_nat where
+  "of_nat json \<equiv> case json of
+    JSON.Nat n \<Rightarrow> Result n
+  | _ \<Rightarrow> Error [STR ''of_nat: expected natural number'']
+" for json
+
+definition of_int where
+  "of_int json \<equiv> case json of
+    JSON.Int n \<Rightarrow> Result n
+  | _ \<Rightarrow> Error [STR ''of_int: expected integral number'']
+" for json
+
+definition [consuming]:
+  "lx_underscore = exactly ''_'' with (\<lambda>_. CHR ''_'')"
+
+definition [consuming]:
+  "lx_hyphen = exactly ''-'' with (\<lambda>_. CHR ''-'')"
+
+definition [consuming]:
+  "ta_var_ident \<equiv>
+    (lx_alphanum \<parallel> lx_underscore)
+    -- Parser_Combinator.repeat (lx_alphanum \<parallel> lx_underscore \<parallel> lx_hyphen)
+    with uncurry (#)
+  "
+
+definition [consuming]:
+  "parse_bound \<equiv> ta_var_ident --
+    exactly ''['' *-- lx_int -- exactly '':'' *-- lx_int --* exactly '']''"
+
+definition "parse_bounds \<equiv> parse_list (lx_ws *-- parse_bound with (\<lambda>(s,p). (String.implode s, p)))"
+
+value [code] "parse parse_bounds (STR ''id[-1:2], id[-1:0]'')"
+
+definition [consuming]:
+  "scan_var = ta_var_ident"
+
+abbreviation seq_ignore_left_ws (infixr "**--" 60)
+  where "p **-- q \<equiv> token p *-- q" for p q
+
+abbreviation seq_ignore_right_ws (infixr "--**" 60)
+  where "p --** q \<equiv> token p --* q" for p q
+
+abbreviation seq_ws (infixr "---" 60)
+  where "seq_ws p q \<equiv> token p -- q" for p q
+
+definition scan_acconstraint where [unfolded Let_def, consuming]:
+  "scan_acconstraint \<equiv>
+    let scan =
+      (\<lambda>s c. scan_var --- exactly s **-- token lx_int with (\<lambda>(x, y). c (String.implode x) y)) in
+  (
+    scan ''<''  lt \<parallel>
+    scan ''<='' le \<parallel>
+    scan ''=''  eq \<parallel>
+    scan ''>='' ge \<parallel>
+    scan ''>''  gt
+  )
+"
+
+definition [consuming]:
+  "scan_parens lparen rparen inner \<equiv> exactly lparen **-- inner --** token (exactly rparen)"
+
+definition [consuming]: "scan_loc \<equiv>
+  (scan_var --- (exactly ''.'' *-- scan_var))
+  with (\<lambda> (p, s). loc (String.implode p) (String.implode s))"
+
+definition [consuming]: "scan_bexp_elem \<equiv> scan_acconstraint \<parallel> scan_loc"
+
+abbreviation "scan_parens' \<equiv> scan_parens ''('' '')''"
+
+definition [consuming]: "scan_infix_pair a b s \<equiv> a --- exactly s **-- token b"
+
+lemma [fundef_cong]:
+  assumes "\<And>l2. ll_fuel l2 \<le> ll_fuel l' \<Longrightarrow> A l2 = A' l2"
+  assumes "\<And>l2. ll_fuel l2 + (if length s > 0 then 1 else 0) \<le> ll_fuel l' \<Longrightarrow> B l2 = B' l2"
+  assumes "s = s'" "l=l'"
+  shows "scan_infix_pair A B s l = scan_infix_pair A' B' s' l'"
+  using assms unfolding scan_infix_pair_def gen_token_def
+  by (cases s; intro Parser_Combinator.bind_cong repeat_cong assms) auto
+
+lemma [fundef_cong]:
+  assumes "\<And>l2. ll_fuel l2 < ll_fuel l \<Longrightarrow> A l2 = A' l2" "l = l'"
+  shows "scan_parens' A l = scan_parens' A' l'"
+  using assms unfolding scan_parens_def gen_token_def
+  by (intro Parser_Combinator.bind_cong repeat_cong assms) auto
+
+fun scan_7 and scan_6 and scan_0 where
+  "scan_7 ::=
+    scan_infix_pair scan_6 scan_7 ''->'' with uncurry imply \<parallel>
+    scan_infix_pair scan_6 scan_7 ''||'' with uncurry sexp.or \<parallel>
+    scan_6" |
+  "scan_6 ::=
+    scan_infix_pair scan_0 scan_6 ''&&'' with uncurry and \<parallel> scan_0" |
+  "scan_0 ::=
+    exactly ''~'' **-- scan_parens' scan_7 with not \<parallel>
+    scan_bexp_elem \<parallel>
+    scan_parens' scan_7"
+
+abbreviation "scan_bexp \<equiv> scan_7"
+
+value [code] "parse scan_bexp (STR ''a < 3 && b>=2 || ~ (c <= 4)'')"
+
+definition [consuming]: "scan_prefix p head = exactly head **-- p" for p
+
+lemma is_cparser_token[parser_rules]:
+  "is_cparser (token a)" if "is_cparser a"
+  using that unfolding gen_token_def by simp
+
+lemma is_cparser_scan_parens'[parser_rules]:
+  "is_cparser (scan_parens' a)"
+  unfolding scan_parens_def by simp
+
+lemma [parser_rules]:
+  "is_cparser scan_0"
+  by (simp add: scan_0.simps[abs_def])
+
+lemma [parser_rules]:
+  "is_cparser scan_6"
+  by (subst scan_6.simps[abs_def]) simp
+
+lemma [parser_rules]:
+  "is_cparser scan_bexp"
+  by (subst scan_7.simps[abs_def]) simp
+
+definition [consuming]: "scan_formula \<equiv>
+  scan_prefix scan_bexp ''E<>'' with formula.EX \<parallel>
+  scan_prefix scan_bexp ''E[]'' with EG \<parallel>
+  scan_prefix scan_bexp ''A<>'' with AX \<parallel>
+  scan_prefix scan_bexp ''A[]'' with AG \<parallel>
+  scan_infix_pair scan_bexp scan_bexp ''-->'' with uncurry Leadsto"
+
+definition [consuming]:
+  "scan_update \<equiv> scan_infix_pair scan_var lx_nat ''='' with (\<lambda>(s, x). (String.implode s, x))"
+
+abbreviation "scan_updates \<equiv> parse_list scan_update"
+
+definition [consuming]: "scan_action \<equiv>
+  (scan_var --* exactly ''?'') with In o String.implode \<parallel>
+  (scan_var --* exactly ''!'') with Out o String.implode \<parallel>
+  scan_var with Sil o String.implode"
+
+abbreviation orelse (infix "orelse" 58) where
+  "a orelse b \<equiv> default b a"
+
+definition
+  "parse_action s \<equiv> parse scan_action s orelse Sil (STR '''')"
+
+(* let scan_edge_label = scan_action <|> str "" ^^ fun _ -> Internal "" *)
+definition assert where "assert b m = (if b then Result () else Error [m])"
+
+fun chop_sexp where
+  "chop_sexp clocks (and a b) (cs, es) =
+    chop_sexp clocks a (cs, es) |> chop_sexp clocks b" |
+  "chop_sexp clocks (eq a b) (cs, es) =
+    (if a \<in> set clocks then (eq a b # cs, es) else (cs, eq a b # es))" |
+  "chop_sexp clocks (le a b) (cs, es) =
+    (if a \<in> set clocks then (lt a b # cs, es) else (cs, eq a b # es))" |
+  "chop_sexp clocks (lt a b) (cs, es) =
+    (if a \<in> set clocks then (eq a b # cs, es) else (cs, eq a b # es))" |
+  "chop_sexp clocks (ge a b) (cs, es) =
+    (if a \<in> set clocks then (eq a b # cs, es) else (cs, eq a b # es))" |
+  "chop_sexp clocks (gt a b) (cs, es) =
+    (if a \<in> set clocks then (eq a b # cs, es) else (cs, eq a b # es))" |
+  "chop_sexp clocks a (cs, es) = (cs, a # es)"
+
+fun sexp_to_acconstraint :: "(String.literal, String.literal, String.literal, int) sexp \<Rightarrow> _" where
+  "sexp_to_acconstraint (lt a (b :: int)) = acconstraint.LT a b" |
+  "sexp_to_acconstraint (le a b) = acconstraint.LE a b" |
+  "sexp_to_acconstraint (eq a b) = acconstraint.EQ a b" |
+  "sexp_to_acconstraint (ge a b) = acconstraint.GE a b" |
+  "sexp_to_acconstraint (gt a b) = acconstraint.GT a b"
+
+no_notation top_assn ("true")
+
+fun sexp_to_bexp :: "(String.literal, String.literal, String.literal, int) sexp \<Rightarrow> _" where
+  "sexp_to_bexp (lt a (b :: int)) = bexp.lt a b |> Result" |
+  "sexp_to_bexp (le a b) = bexp.le a b |> Result" |
+  "sexp_to_bexp (eq a b) = bexp.eq a b |> Result" |
+  "sexp_to_bexp (ge a b) = bexp.ge a b |> Result" |
+  "sexp_to_bexp (gt a b) = bexp.gt a b |> Result" |
+  "sexp_to_bexp (and a b) =
+    do {a \<leftarrow> sexp_to_bexp a; b \<leftarrow> sexp_to_bexp b; bexp.and a b |> Result}" |
+  "sexp_to_bexp (sexp.or a b) =
+    do {a \<leftarrow> sexp_to_bexp a; b \<leftarrow> sexp_to_bexp b; bexp.or a b |> Result}" |
+  "sexp_to_bexp (imply a b) =
+    do {a \<leftarrow> sexp_to_bexp a; b \<leftarrow> sexp_to_bexp b; bexp.imply a b |> Result}" |
+  "sexp_to_bexp x        = Error [STR ''Illegal construct in binary operation'']"
+
+definition true where "true \<equiv> sexp.or (gt (STR ''a'') 1) (le (STR ''a'') 1)"
+
+definition true_bexp where "true_bexp \<equiv> bexp.or (bexp.gt (STR ''a'') 1) (bexp.le (STR ''a'') 1)"
+
+derive "show" bexp
+
+instantiation String.literal :: "show"
+begin
+
+definition "shows_prec p (s::String.literal) rest = String.explode s @ rest" for p
+definition "shows_list (cs::String.literal list) s = concat (map String.explode cs) @ s"
+instance
+  by standard (simp_all add: shows_prec_literal_def shows_list_literal_def show_law_simps)
+
+end
+
+definition compile_invariant where
+  "compile_invariant clocks vars inv \<equiv>
+    let
+      (cs, es) = chop_sexp clocks inv ([], []);
+      g = map sexp_to_acconstraint cs;
+      e = (if es = [] then true else fold (and) (tl es) (hd es))
+    in do {
+      b \<leftarrow> sexp_to_bexp e;
+      assert (set1_bexp b \<subseteq> set vars) (String.implode (''Unknown variable in bexp: '' @ show b));
+      Result (g, b)
+    }
+  " for inv
+
+definition convert_node where
+  "convert_node clocks vars n \<equiv> do {
+    n \<leftarrow>  of_object n;
+    ID \<leftarrow> get n ''id'' \<bind> of_nat;
+    name \<leftarrow> get n ''name'' \<bind> of_string;
+    inv \<leftarrow> get n ''invariant'' \<bind> of_string;
+    (inv, inv_vars) \<leftarrow> (
+      if inv = STR ''''
+      then Result ([], true_bexp)
+      else do {
+        inv \<leftarrow> parse scan_bexp inv |> err_msg (STR ''Failed to parse invariant in '' + inv);
+        compile_invariant clocks vars inv
+    });
+    assert (inv_vars = true_bexp) (STR ''State invariants on nodes are not supported'');
+    Result ((name, ID), inv)
+  }"
+
+definition convert_edge where
+  "convert_edge clocks vars e \<equiv> do {
+    e \<leftarrow> of_object e;
+    source \<leftarrow> get e ''source'' \<bind> of_nat;
+    target \<leftarrow> get e ''target'' \<bind> of_nat;
+    guard  \<leftarrow> get e ''guard''  \<bind> of_string;
+    label  \<leftarrow> get e ''label''  \<bind> of_string;
+    update \<leftarrow> get e ''update'' \<bind> of_string;
+    label  \<leftarrow> parse scan_action label |> err_msg (STR ''Failed to parse label in '' + label);
+    guard  \<leftarrow> parse scan_bexp guard |> err_msg (STR ''Failed to parse guard in '' + guard);
+    (g, _) \<leftarrow> compile_invariant clocks vars guard;
+    update \<leftarrow> parse scan_updates update |> err_msg (STR ''Failed to parse update in '' + update);
+    let resets = filter (\<lambda>x. fst x \<in> set clocks) update;
+    assert
+      (list_all (\<lambda>(_, d). d = 0) resets)
+      (STR ''Clock resets to values different from zero are not supported'');
+    let resets = map fst resets;
+    let upds = filter (\<lambda>x. fst x \<notin> set clocks) update;
+    assert
+      (list_all (\<lambda>(x, _). x \<in> set vars) upds)
+      (STR ''Unknown variable in update'');
+    let upds = map (\<lambda>(x, d). (x, (exp.const (int d) :: (String.literal, int) exp))) upds;
+    Result (source, g, label, upds, resets, target)
+  }"
+
+definition convert_automaton where
+  "convert_automaton clocks vars a \<equiv> do {
+    nodes \<leftarrow> get a ''nodes'' \<bind> of_array;
+    edges \<leftarrow> get a ''edges'' \<bind> of_array;
+    nodes \<leftarrow> combine_map (convert_node clocks vars) nodes;
+    let invs = map (\<lambda> ((_, n), g). (n, g)) nodes;
+    let names_to_ids = map fst nodes;
+    assert (distinct (map fst names_to_ids)) (STR ''Node names are ambiguous'');
+    assert (distinct (map snd names_to_ids)) (STR ''Duplicate node id'');
+    let names_to_ids = map_of names_to_ids;
+    let commited = default (STR '''') (get a ''commited'' \<bind> of_string);
+    commited \<leftarrow> parse (parse_list (token ta_var_ident with String.implode)) commited;
+    commited \<leftarrow> combine_map (get names_to_ids) commited;
+    edges \<leftarrow> combine_map (convert_edge clocks vars) edges;
+    Result (names_to_ids, (commited, edges, invs))
+  }"
+
+fun rename_locs_sexp where
+  "rename_locs_sexp f (not a) =
+    do {a \<leftarrow> rename_locs_sexp f a; not a |> Result}" |
+  "rename_locs_sexp f (imply a b) =
+    do {a \<leftarrow> rename_locs_sexp f a; b \<leftarrow> rename_locs_sexp f b; imply a b |> Result}" |
+  "rename_locs_sexp f (sexp.or a b) =
+    do {a \<leftarrow> rename_locs_sexp f a; b \<leftarrow> rename_locs_sexp f b; sexp.or a b |> Result}" |
+  "rename_locs_sexp f (and a b) =
+    do {a \<leftarrow> rename_locs_sexp f a; b \<leftarrow> rename_locs_sexp f b; and a b |> Result}" |
+  "rename_locs_sexp f (loc n x) = do {x \<leftarrow> f n x; loc n x |> Result}" |
+  "rename_locs_sexp f (eq a b) = Result (eq a b)" |
+  "rename_locs_sexp f (lt a b) = Result (lt a b)" |
+  "rename_locs_sexp f (le a b) = Result (le a b)" |
+  "rename_locs_sexp f (ge a b) = Result (ge a b)" |
+  "rename_locs_sexp f (gt a b) = Result (gt a b)"
+
+fun rename_locs_formula where
+  "rename_locs_formula f (formula.EX \<phi>) = rename_locs_sexp f \<phi> \<bind> Result o formula.EX" |
+  "rename_locs_formula f (EG \<phi>) = rename_locs_sexp f \<phi> \<bind> Result o EG" |
+  "rename_locs_formula f (AX \<phi>) = rename_locs_sexp f \<phi> \<bind> Result o AX" |
+  "rename_locs_formula f (AG \<phi>) = rename_locs_sexp f \<phi> \<bind> Result o AG" |
+  "rename_locs_formula f (Leadsto \<phi> \<psi>) =
+    do {\<phi> \<leftarrow> rename_locs_sexp f \<phi>; \<psi> \<leftarrow> rename_locs_sexp f \<psi>; Leadsto \<phi> \<psi> |> Result}"
+
+definition convert :: "JSON \<Rightarrow>
+  (String.literal list \<times>
+    (nat list \<times>
+     (String.literal act, nat, String.literal, int, String.literal, int) transition list
+      \<times> (nat \<times> (String.literal, int) cconstraint) list) list \<times>
+   (String.literal \<times> int \<times> int) list \<times> (nat, nat, String.literal, int) formula
+  ) Error_List_Monad.result" where
+  "convert json \<equiv> do {
+    all \<leftarrow> of_object json;
+    automata \<leftarrow> get all ''automata'';
+    automata \<leftarrow> of_array automata;
+    let broadcast = default [] (do {
+      x \<leftarrow> get all ''broadcast''; of_array x}
+    );
+    broadcast \<leftarrow> combine_map of_string broadcast;
+    let bounds = default (STR '''') (do {
+      x \<leftarrow> get all ''vars''; of_string x}
+    );
+    bounds \<leftarrow> parse parse_bounds bounds;
+    clocks \<leftarrow> get all ''clocks'';
+    clocks \<leftarrow> of_string clocks;
+    clocks \<leftarrow> parse (parse_list (lx_ws *-- ta_var_ident with String.implode)) clocks;
+    formula \<leftarrow> get all ''formula'';
+    formula \<leftarrow> of_string formula;
+    formula \<leftarrow> parse scan_formula formula;
+    automata \<leftarrow> combine_map of_object automata;
+    process_names \<leftarrow> combine_map (\<lambda>a. get a ''name'' \<bind> of_string) automata;
+    assert (distinct process_names) (STR ''Process names are ambiguous'');
+    let process_names_to_index = List_Index.index process_names;
+    init_locs \<leftarrow> combine_map
+      (\<lambda>a. do {x \<leftarrow> get a ''initial''; x \<leftarrow> of_nat x; show x |> String.implode |> Result})
+      automata;
+    let formula = formula.map_formula process_names_to_index id id id formula;
+    let vars = map fst bounds;
+    names_automata \<leftarrow> combine_map (convert_automaton clocks vars) automata;
+    let automata = map snd names_automata;
+    let names    = map fst names_automata;
+    formula \<leftarrow> rename_locs_formula (\<lambda>i. get (names ! i)) formula;
+    Result (broadcast, automata, bounds, formula)
+}" for json
+
+
+
+paragraph \<open>Unsafe Glue Code for Printing\<close>
+
+definition print :: "String.literal \<Rightarrow> unit" where
+  "print x = ()"
+
+code_printing
+  constant print \<rightharpoonup> (SML) "print _"
+       and        (OCaml) "print'_string _"
+
+definition println :: "String.literal \<Rightarrow> unit" where
+  "println x = print (x + STR ''\<newline>'')"
+
+definition "print_err = print"
+definition "println_err x = print_err (x + STR ''\<newline>'')"
+
+definition parse_convert_run_print where
+  "parse_convert_run_print s \<equiv>
+   case parse json s \<bind> convert of
+     Error es \<Rightarrow> do {let _ = map println es; return ()}
+   | Result (broadcast, automata, bounds, formula) \<Rightarrow> do {
+      r \<leftarrow> do_preproc_mc (broadcast, automata, bounds) [] [] formula;
+      case r of
+        Error es \<Rightarrow> do {let _ = map println es; return ()}
+      | Result s \<Rightarrow> do {let _ = println s; return ()}
+  }"
+
+export_code do_preproc_mc checking SML
+
+export_code parse_convert_run_print in SML_imp module_name Test
+
+text \<open>A small test of parsing + conversion:\<close>
+definition "parse_convert_run s \<equiv> parse json s \<bind> convert"
+
+ML \<open>
+  fun test file =
+  let
+    val s = file_to_string file;
+  in
+    @{code parse_convert_run} s end
+\<close>
+
+ML_val \<open>test "../benchmarks/HDDI_02.muntax"\<close>
 
 end
