library/Error_List_Monad.thy
@@ -1,0 +1,63 @@
+theory Error_List_Monad
+  imports Main "HOL-Library.Monad_Syntax"
+begin
+
+
+(* Error monad *)
+type_synonym error = String.literal
+
+datatype 'a result =
+  is_result: Result 'a
+| is_error:  Error "error list"
+
+fun bind where "bind m f = (case m of
+  Result x \<Rightarrow> f x
+| Error es \<Rightarrow> Error es)"
+
+adhoc_overloading "Monad_Syntax.bind" bind
+
+fun err_msg where
+  "err_msg m (Error es) = Error (m # es)"
+| "err_msg m x = x"
+
+fun make_err where
+  "make_err m (Error es) = Error (es @ [m])"
+| "make_err m _ = Error [m]"
+
+definition assert_msg where "assert_msg b m = (if b then (\<lambda>x. x) else make_err m)"
+
+fun the_result where
+  "the_result (Result x) = x"
+
+fun the_errors where
+  "the_errors (Error es) = es"
+
+fun combine2_gen where
+  "combine2_gen comb (Error e1) (Error e2) = Error (List.append e1 e2)"
+| "combine2_gen comb (Error e)  (Result _) = Error e"
+| "combine2_gen comb (Result _) (Error e)  = Error e"
+| "combine2_gen comb (Result a) (Result b) = comb a b"
+
+(* let combine2: ('a result * 'b result -> ('a * 'b) result) = combine2_gen (fun a b -> Result (a, b)) *)
+
+definition "combine2 = combine2_gen (\<lambda>a b. Result (a, b))"
+
+notation combine2 (infixr "<|>" 60)
+
+fun combine where
+  "combine [] = Result []"
+| "combine (x # xs) = combine2_gen (\<lambda>x xs. Result (x # xs)) x (combine xs)"
+
+abbreviation (input) app (infixl "|>" 59) where "a |> b \<equiv> b a"
+
+definition "combine_map f xs = List.map f xs |> combine"
+
+fun map_errors where
+  "map_errors f (Error errors) = Error (List.map f errors)"
+| "map_errors f r = r"
+
+fun fold_error where
+  "fold_error f [] a = Result a"
+| "fold_error f (x # xs) a = do {a \<leftarrow> f x a; fold_error f xs a}"
+
+end
